Fifo/Ifc.v
@@ -1,25 +1,24 @@
 Require Import Kami.AllNotations.
-Section FifoInterface.
-  Class FifoParams :=
+
+Section Ifc.
+  Class Params := { name: string;
+                    k: Kind;
+                    size: nat;
+                    lgSize := Nat.log2_up size ;
+                    }.
+
+  Context {params: Params}.
+
+  Record Ifc: Type :=
     {
-      name: string;
-      k : Kind;
+      regs: list RegInitT;
+      regFiles: list RegFileBase;
+      isEmpty: forall {ty}, ActionT ty Bool;
+      isFull: forall {ty}, ActionT ty Bool;
+      numFree: forall {ty}, ActionT ty (Bit lgSize);
+      first: forall {ty}, ActionT ty (Maybe k);
+      deq: forall {ty}, ActionT ty (Maybe k);
+      enq: forall {ty}, ty k -> ActionT ty Bool;
+      flush: forall {ty}, ActionT ty Void
     }.
-
-  Section fifoParams.
-    Context (fifoParams: FifoParams). 
-
-    Record Fifo: Type :=
-      {
-        getLen: nat;
-        regs: list RegInitT;
-        regFiles: list RegFileBase;
-        isEmpty: forall {ty}, ActionT ty Bool;
-        isFull: forall {ty}, ActionT ty Bool;
-        first: forall {ty}, ActionT ty (Maybe k);
-        deq: forall {ty}, ActionT ty (Maybe k);
-        enq: forall {ty}, ty k -> ActionT ty Bool;
-        flush: forall {ty}, ActionT ty Void
-      }.
-  End fifoParams.
-End FifoInterface.
+End Ifc.
