FreeList/Fifo.v
@@ -2,75 +2,72 @@ Require Import Kami.AllNotations.
 Require Import StdLibKami.Fifo.Ifc.
 Require Import StdLibKami.FreeList.Ifc.
 
-Section ImplTagFreeList.
-  Context {freeListParams : FreeListParams}.
+Section Impl.
+  Context {ifcParams : Ifc.Params}.
+  
+  Context (fifo: @Fifo.Ifc.Ifc {| Fifo.Ifc.name := (name ++ ".fifo")%string;
+                                  Fifo.Ifc.k    := Bit lgSize;
+                                  Fifo.Ifc.size := size;
+                               |}).
+  
+  Local Definition Tag := Bit lgSize.
+
+  Local Open Scope kami_expr.
+  Local Open Scope kami_action.
 
   Local Definition initName := (name ++ ".initTag")%string.
 
-  Section withParams.
-    Context (backingFifo: @Fifo ({|
-                                    StdLibKami.Fifo.Ifc.name := (StdLibKami.FreeList.Ifc.name ++ ".backingFifo")%string;
-                                    StdLibKami.Fifo.Ifc.k    := Bit tagSz
-                                  |})).
-    
-    Local Definition Tag := Bit tagSz.
-
-    Local Open Scope kami_expr.
-    Local Open Scope kami_action.
-
-    Local Definition initNotDone ty: ActionT ty (Maybe Tag) := (
-      Read init: Tag <- initName;
-      LET initNotDone: Bool <- (ZeroExtendTruncMsb _ #init: Bit 1 @# ty) != $1;
-      Ret (STRUCT { "valid" ::= #initNotDone;
-                    "data" ::= #init }: Maybe Tag @# ty)).
-    
-    (* Initialization rule, which will fill the free list *)
-    Local Definition initialize ty: ActionT ty Void := (
-      LETA initNotDone: Maybe Tag <- initNotDone _;
-      LET initNotDoneData <- #initNotDone @% "data";
-      If ((#initNotDone @% "valid")) then (
-          LETA _ <- (@Ifc.enq _ backingFifo ty) initNotDoneData;
-          Write initName: Tag <- #initNotDoneData + $1;
-          Retv
-        );
-      Retv).
-
-    Local Definition nextToAlloc ty: ActionT ty (Maybe Tag) := (
-      LETA initNotDone: Maybe Tag <- initNotDone _;
-      LETA first: Maybe Tag <- (@Ifc.first _ backingFifo ty);
-      LET res: Maybe Tag <- STRUCT { "valid" ::= (!(#initNotDone @% "valid") && (#first @% "valid")) ;
-                                     "data" ::= #first @% "data" };
-      Ret #res).
+  Local Definition initNotDone ty: ActionT ty (Maybe Tag) := (
+    Read init: Tag <- initName;
+    LET initNotDone: Bool <- #init != $size;
+    Ret (STRUCT { "valid" ::= #initNotDone;
+                  "data" ::= #init }: Maybe Tag @# ty)).
   
-    Local Definition alloc ty (tag: ty Tag): ActionT ty Bool := (
-      LETA initNotDone: Maybe Tag <- initNotDone _;
-      LETA first: Maybe Tag <- (@Ifc.first _ backingFifo ty);
-      LET doDequeue: Bool <- !(#initNotDone @% "valid") && #first @% "valid" && (#tag == #first @% "data");
-      If #doDequeue then (
-          LETA _: Maybe Tag <- (@Ifc.deq _ backingFifo ty);
-          Retv
-        );
-      Ret #doDequeue).
-  
-    Local Definition free ty (tag: ty Tag): ActionT ty Void := (
-      LETA initNotDone: Maybe Tag <- initNotDone _;
-      If !(#initNotDone @% "valid") then (
-          LETA _ <- (@Ifc.enq _ backingFifo ty) tag;
-          Retv
+  (* Initialization rule, which will fill the free list *)
+  Local Definition initialize ty: ActionT ty Void := (
+    LETA initNotDone: Maybe Tag <- initNotDone _;
+    LET initNotDoneData <- #initNotDone @% "data";
+    If ((#initNotDone @% "valid")) then (
+        LETA _ <- (@Ifc.enq _ fifo ty) initNotDoneData;
+        Write initName: Tag <- #initNotDoneData + $1;
+        Retv
       );
-      Retv).
-    
-    Local Definition regs: list RegInitT := makeModule_regs ( Register initName: Tag <- $ 0 )%kami ++ (@Fifo.Ifc.regs _ backingFifo).
-    
-    Definition fifoFreeList: FreeList :=
-      {|
-        FreeList.Ifc.regs := regs;
-        FreeList.Ifc.regFiles := @Fifo.Ifc.regFiles _ backingFifo;
-        FreeList.Ifc.length := Nat.pow 2 tagSz;
-        FreeList.Ifc.initialize := initialize;
-        FreeList.Ifc.nextToAlloc := nextToAlloc;
-        FreeList.Ifc.alloc := alloc;
-        FreeList.Ifc.free := free
-      |}.
-  End withParams.
-End ImplTagFreeList.
+    Retv).
+
+  Local Definition nextToAlloc ty: ActionT ty (Maybe Tag) := (
+    LETA initNotDone: Maybe Tag <- initNotDone _;
+    LETA first: Maybe Tag <- (@Ifc.first _ fifo ty);
+    LET res: Maybe Tag <- STRUCT { "valid" ::= (!(#initNotDone @% "valid") && (#first @% "valid")) ;
+                                   "data" ::= #first @% "data" };
+    Ret #res).
+
+  Local Definition alloc ty (tag: ty Tag): ActionT ty Bool := (
+    LETA initNotDone: Maybe Tag <- initNotDone _;
+    LETA first: Maybe Tag <- (@Ifc.first _ fifo ty);
+    LET doDequeue: Bool <- !(#initNotDone @% "valid") && #first @% "valid" && (#tag == #first @% "data");
+    If #doDequeue then (
+        LETA _: Maybe Tag <- (@Ifc.deq _ fifo ty);
+        Retv
+      );
+    Ret #doDequeue).
+
+  Local Definition free ty (tag: ty Tag): ActionT ty Void := (
+    LETA initNotDone: Maybe Tag <- initNotDone _;
+    If !(#initNotDone @% "valid") then (
+        LETA _ <- (@Ifc.enq _ fifo ty) tag;
+        Retv
+    );
+    Retv).
+  
+  Local Definition regs: list RegInitT := makeModule_regs ( Register initName: Tag <- $ 0 )%kami ++ (@Fifo.Ifc.regs _ fifo).
+  
+  Definition impl: Ifc :=
+    {|
+      Ifc.regs := regs;
+      Ifc.regFiles := Fifo.Ifc.regFiles fifo;
+      Ifc.initialize := initialize;
+      Ifc.nextToAlloc := nextToAlloc;
+      Ifc.alloc := alloc;
+      Ifc.free := free
+    |}.
+End Impl.
