FreeList/Spec.v
@@ -1,55 +1,51 @@
 Require Import Kami.AllNotations.
 Require Import StdLibKami.FreeList.Ifc.
 Section FreeListSpec.
-  Context {freeListParams : FreeListParams}.
+  Context {ifcParams : Ifc.Params}.
 
   Local Definition arrayRegName := (name ++ ".data")%string.
 
-  Section withParams.    
-    Local Definition len := Nat.pow 2 tagSz.
-    Local Definition Tag := Bit tagSz.
+  Local Definition Tag := Bit lgSize.
 
-    Local Open Scope kami_expr.
-    Local Open Scope kami_action.
+  Local Open Scope kami_expr.
+  Local Open Scope kami_action.
 
-    Local Definition initialize ty: ActionT ty Void :=
-      Write arrayRegName: Array len Bool <- BuildArray (fun _ => $$false);
-      Retv.
+  Local Definition initialize ty: ActionT ty Void :=
+    Write arrayRegName: Array size Bool <- BuildArray (fun _ => $$false);
+    Retv.
 
-    Local Definition nextToAlloc ty: ActionT ty (Maybe Tag) := 
-      Read freeArray: Array len Bool <- arrayRegName;
-      Nondet random: Tag;
-      LET randomOk: Bool <- #freeArray@[#random];
-      LET res: Maybe Tag <- STRUCT { "valid" ::= !#randomOk;
-                                     "data" ::= #random };
-      Ret #res.
-  
-    Local Definition alloc ty (tag: ty Tag): ActionT ty Bool := 
-      Read freeArray: Array len Bool <- arrayRegName;
-      LET res: Bool <- #freeArray@[#tag];
-      Write arrayRegName: Array len Bool <- #freeArray@[#tag <- $$true];
-      Ret !#res.
-  
-    Local Definition free ty (tag: ty Tag): ActionT ty Void :=
-      Read freeArray: Array len Bool <- arrayRegName;                                                        
-      Write arrayRegName: Array len Bool <- #freeArray@[#tag <- $$false];
-      Retv.
+  Local Definition nextToAlloc ty: ActionT ty (Maybe Tag) := 
+    Read freeArray: Array size Bool <- arrayRegName;
+    Nondet random: Tag;
+    LET randomOk: Bool <- #freeArray@[#random];
+    LET res: Maybe Tag <- STRUCT { "valid" ::= !#randomOk;
+                                   "data" ::= #random };
+    Ret #res.
 
-    Local Definition regs: list RegInitT := makeModule_regs ( Register arrayRegName: Array len Bool <- Default )%kami.
+  Local Definition alloc ty (tag: ty Tag): ActionT ty Bool := 
+    Read freeArray: Array size Bool <- arrayRegName;
+    LET res: Bool <- #freeArray@[#tag];
+    Write arrayRegName: Array size Bool <- #freeArray@[#tag <- $$true];
+    Ret !#res.
 
-    Definition specFreeList: FreeList := 
-      {|
-        FreeList.Ifc.regs := regs;
-        FreeList.Ifc.regFiles := nil;
-        FreeList.Ifc.length := len;
-        FreeList.Ifc.initialize := initialize;
-        FreeList.Ifc.nextToAlloc := nextToAlloc;
-        FreeList.Ifc.alloc := alloc;
-        FreeList.Ifc.free := free
-      |}.
-        
-    Local Close Scope kami_action.
-    Local Close Scope kami_expr.
+  Local Definition free ty (tag: ty Tag): ActionT ty Void :=
+    Read freeArray: Array size Bool <- arrayRegName;                                                        
+    Write arrayRegName: Array size Bool <- #freeArray@[#tag <- $$false];
+    Retv.
 
-  End withParams.
+  Local Definition regs: list RegInitT := makeModule_regs ( Register arrayRegName: Array size Bool <- Default )%kami.
+
+  Definition impl: Ifc := 
+    {|
+      Ifc.regs := regs;
+      Ifc.regFiles := nil;
+      Ifc.initialize := initialize;
+      Ifc.nextToAlloc := nextToAlloc;
+      Ifc.alloc := alloc;
+      Ifc.free := free
+    |}.
+      
+  Local Close Scope kami_action.
+  Local Close Scope kami_expr.
+
 End FreeListSpec.
