ReplacementPolicy/PseudoLru.v
@@ -1,16 +1,15 @@
-(* Implements the Pseudo Least Recently Used Algorithm. *)
 Require Import Kami.AllNotations.
 Require Import StdLibKami.ReplacementPolicy.Ifc.
 
 Section lru.
-  Context {policyParams : PolicyParams}.
+  Context {ifcParams : Params}.
 
-  Local Definition stateRegName := (StdLibKami.ReplacementPolicy.Ifc.name ++ ".state")%string.
+  Local Definition replacementName := (ReplacementPolicy.Ifc.name ++ ".state")%string.
 
   (* Variable params: PseudoLruParams. *)
   
-  Local Definition State := Array (num - 1) Bool.
-  Local Definition IndexWidth := Nat.log2_up num.
+  Local Definition State := Array (size - 1) Bool.
+  Local Definition IndexWidth := Nat.log2_up size.
   Local Definition Index := Bit IndexWidth.
   Local Definition PathWidth := IndexWidth.
   Local Definition Path := Index.
@@ -21,8 +20,8 @@ Section lru.
   Section ty.
     Variable ty : Kind -> Type.
     
-    Local Definition leftOverNum := num - Nat.pow 2 (Nat.log2 num).
-    Local Definition twiceLeftOverNum := 2*leftOverNum.
+    Local Definition leftOverSize := size - Nat.pow 2 (Nat.log2 size).
+    Local Definition twiceLeftOverSize := 2*leftOverSize.
 
     Local Open Scope kami_expr.
     Local Open Scope kami_action.
@@ -31,18 +30,18 @@ Section lru.
     Local Definition div2 n (v: Bit n @# ty) := (v >> ($1: Bit 1 @# ty)). 
     Local Definition mod2 n (v: Bit n @# ty) := (v .& $1).
 
-    Local Definition getPathFromIndex (i: Index @# ty) := match leftOverNum with
+    Local Definition getPathFromIndex (i: Index @# ty) := match leftOverSize with
                                                           | 0 => i
-                                                          | _ => (IF i < $twiceLeftOverNum
+                                                          | _ => (IF i < $twiceLeftOverSize
                                                                   then i
-                                                                  else mul2 (i - $leftOverNum))
+                                                                  else mul2 (i - $leftOverSize))
                                                           end.
 
-    Local Definition getIndexFromPath (p: Path @# ty) := match leftOverNum with
+    Local Definition getIndexFromPath (p: Path @# ty) := match leftOverSize with
                                                          | 0 => p
-                                                         | _ => (IF p < $twiceLeftOverNum
+                                                         | _ => (IF p < $twiceLeftOverSize
                                                                  then p
-                                                                 else div2 p + $leftOverNum)
+                                                                 else div2 p + $leftOverSize)
                                                          end.
 
     Section state.
@@ -50,7 +49,7 @@ Section lru.
       Local Fixpoint getVictimAux (depth: nat) (i: TreeIndex @# ty) (p: Path @# ty): Path ## ty :=
         match depth with
         | 0 => RetE p
-        | S m => (IfE i >= $(num-1)
+        | S m => (IfE i >= $(size-1)
                   then RetE (mul2 p)
                   else (LETC direction : Bool <- state@[i];
                           LETC newIndex : TreeIndex <- mul2 i + IF #direction then $2 else $1;
@@ -69,7 +68,7 @@ Section lru.
       Local Fixpoint accessAux (depth: nat) (i: TreeIndex @# ty) (s: State @# ty): State ## ty :=
         match depth with
         | 0 => RetE s
-        | S m => (IfE i >= $(num-1)
+        | S m => (IfE i >= $(size-1)
                   then RetE s
                   else (LETC direction: Bool <- (* pathToArray@[$$ (natToWord (Nat.log2_up PathWidth) m)] *) ((path >> ($m: Bit PathWidth @# ty)) .& $1) == $1;
                           LETC newIndex : TreeIndex <- mul2 i + (IF #direction then $2 else $1);
@@ -84,19 +83,20 @@ Section lru.
   Local Open Scope kami_expr.
   Local Open Scope kami_action.
   
-  Definition PseudoLru
-    :  @ReplacementPolicy policyParams
+  Definition impl : Ifc
     := {|
+        regs := makeModule_regs (Register replacementName: State <- Default)%kami;
+        regFiles := nil;
         getVictim := (fun ty =>
-                        Read state : State <- stateRegName;
-                          LETA path : Path <- convertLetExprSyntax_ActionT
-                                           (getVictimAux #state Depth $0 $0);
-                          Ret (getIndexFromPath #path));
+                        Read state : State <- replacementName;
+                        LETA path : Path <- convertLetExprSyntax_ActionT
+                                              (getVictimAux #state Depth $0 $0);
+                        Ret (getIndexFromPath #path));
         access := (fun ty index =>
-                     Read state : State <- stateRegName;
-                       LETA result : State <- convertLetExprSyntax_ActionT (accessAux (getPathFromIndex index) Depth $0 #state);
-                       Write stateRegName : State <- #result;
-                       Retv)
+                     Read state : State <- replacementName;
+                     LETA result : State <- convertLetExprSyntax_ActionT (accessAux (getPathFromIndex index) Depth $0 #state);
+                     Write replacementName : State <- #result;
+                     Retv)
       |}.
 
   Local Close Scope kami_action.
@@ -111,36 +111,38 @@ Section tests.
   Local Notation L := (Const type false).
   Local Notation R := (Const type true).
 
-  Definition testGetVictim (num : nat)
+  Definition testGetVictim (size : nat)
     := let params
-         :  PolicyParams
+         : Params
          := {|
-              StdLibKami.ReplacementPolicy.Ifc.name := "test";
-              StdLibKami.ReplacementPolicy.Ifc.num  := num;
+              ReplacementPolicy.Ifc.name := "test";
+              ReplacementPolicy.Ifc.size  := size;
             |} in
        fun (state: State @# type) (expected : word IndexWidth) =>
          (evalLetExpr (LETE path : Path <- getVictimAux state Depth $0 $0;
                          RetE (getIndexFromPath (Var _ (SyntaxKind _) path))) = expected).
-  Open Scope word.
-  Goal testGetVictim (num := 3) (ARRAY {R; R}) $2. Proof. reflexivity. Qed.
-  Goal testGetVictim (num := 3) (ARRAY {R; L}) $2. Proof. reflexivity. Qed.
-  Goal testGetVictim (num := 3) (ARRAY {L; R}) $1. Proof. reflexivity. Qed.
 
-  Goal testGetVictim (num := 6) (ARRAY {R; R; R; R; R}) $5. Proof. reflexivity. Qed.
-  Goal testGetVictim (num := 6) (ARRAY {L; R; R; R; R}) $3. Proof. reflexivity. Qed.
-  Goal testGetVictim (num := 6) (ARRAY {L; R; L; R; R}) $3. Proof. reflexivity. Qed.
-  Goal testGetVictim (num := 6) (ARRAY {R; L; R; R; L}) $5. Proof. reflexivity. Qed.
-  Goal testGetVictim (num := 6) (ARRAY {R; L; R; R; R}) $5. Proof. reflexivity. Qed.
-  Goal testGetVictim (num := 6) (ARRAY {R; R; R; L; R}) $5. Proof. reflexivity. Qed.
+  Local Open Scope word.
+  Goal testGetVictim (size := 3) (ARRAY {R; R}) $2. Proof. reflexivity. Qed.
+  Goal testGetVictim (size := 3) (ARRAY {R; L}) $2. Proof. reflexivity. Qed.
+  Goal testGetVictim (size := 3) (ARRAY {L; R}) $1. Proof. reflexivity. Qed.
+
+  Goal testGetVictim (size := 6) (ARRAY {R; R; R; R; R}) $5. Proof. reflexivity. Qed.
+  Goal testGetVictim (size := 6) (ARRAY {L; R; R; R; R}) $3. Proof. reflexivity. Qed.
+  Goal testGetVictim (size := 6) (ARRAY {L; R; L; R; R}) $3. Proof. reflexivity. Qed.
+  Goal testGetVictim (size := 6) (ARRAY {R; L; R; R; L}) $5. Proof. reflexivity. Qed.
+  Goal testGetVictim (size := 6) (ARRAY {R; L; R; R; R}) $5. Proof. reflexivity. Qed.
+  Goal testGetVictim (size := 6) (ARRAY {R; R; R; L; R}) $5. Proof. reflexivity. Qed.
   
-  Goal testGetVictim (num := 7) (ARRAY {R; R; R; R; R; R}) $6. Proof. reflexivity. Qed.
-  Goal testGetVictim (num := 7) (ARRAY {R; R; R; L; R; R}) $6. Proof. reflexivity. Qed.
-  Goal testGetVictim (num := 7) (ARRAY {R; L; L; R; R; R}) $5. Proof. reflexivity. Qed.
-  Goal testGetVictim (num := 7) (ARRAY {R; L; R; R; L; R}) $6. Proof. reflexivity. Qed.
-  Goal testGetVictim (num := 7) (ARRAY {L; R; R; R; R; R}) $3. Proof. reflexivity. Qed.
-  Goal testGetVictim (num := 7) (ARRAY {L; R; R; R; R; L}) $3. Proof. reflexivity. Qed.
-  Goal testGetVictim (num := 7) (ARRAY {L; R; L; R; R; R}) $3. Proof. reflexivity. Qed.
-  Close Scope word.
+  Goal testGetVictim (size := 7) (ARRAY {R; R; R; R; R; R}) $6. Proof. reflexivity. Qed.
+  Goal testGetVictim (size := 7) (ARRAY {R; R; R; L; R; R}) $6. Proof. reflexivity. Qed.
+  Goal testGetVictim (size := 7) (ARRAY {R; L; L; R; R; R}) $5. Proof. reflexivity. Qed.
+  Goal testGetVictim (size := 7) (ARRAY {R; L; R; R; L; R}) $6. Proof. reflexivity. Qed.
+  Goal testGetVictim (size := 7) (ARRAY {L; R; R; R; R; R}) $3. Proof. reflexivity. Qed.
+  Goal testGetVictim (size := 7) (ARRAY {L; R; R; R; R; L}) $3. Proof. reflexivity. Qed.
+  Goal testGetVictim (size := 7) (ARRAY {L; R; L; R; R; R}) $3. Proof. reflexivity. Qed.
+  Local Close Scope word.
+  
   Definition evalArray
     (k : Kind)
     (n : nat)
@@ -148,23 +150,23 @@ Section tests.
     :  list (type k)
     := map (evalLetExpr arr) (getFins n).
 
-  Definition testAccess (num : nat) :=
+  Definition testAccess (size : nat) :=
     let params
-      :  PolicyParams
+      : Params
       := {|
-           StdLibKami.ReplacementPolicy.Ifc.name := "test";
-           StdLibKami.ReplacementPolicy.Ifc.num  := num;
+           ReplacementPolicy.Ifc.name := "test";
+           ReplacementPolicy.Ifc.size  := size;
          |} in
     fun (state: State @# type) (index: Index @# type) (expected : list bool) =>
       evalArray (accessAux (getPathFromIndex index) Depth $0 state) = expected.
 
-  Goal testAccess (num := 2) (ARRAY {R}) (Const type (1'b"0")) [true]. Proof. reflexivity. Qed.
-  Goal testAccess (num := 2) (ARRAY {R}) (Const type (1'b"1")) [false]. Proof. reflexivity. Qed.
+  Goal testAccess (size := 2) (ARRAY {R}) (Const type (1'b"0")) [true]. Proof. reflexivity. Qed.
+  Goal testAccess (size := 2) (ARRAY {R}) (Const type (1'b"1")) [false]. Proof. reflexivity. Qed.
   
-  Goal testAccess (num := 3) (ARRAY {R; R}) (Const type (2'b"01")) [true; false]. Proof. reflexivity. Qed.
-  Goal testAccess (num := 3) (ARRAY {R; R}) (Const type (2'b"00")) [true; true]. Proof. reflexivity. Qed.
-  Goal testAccess (num := 3) (ARRAY {R; R}) (Const type (2'b"10")) [false; true]. Proof. reflexivity. Qed.
-  Goal testAccess (num := 3) (ARRAY {R; R}) (Const type (2'b"11")) [true; true]. Proof. reflexivity. Qed.
+  Goal testAccess (size := 3) (ARRAY {R; R}) (Const type (2'b"01")) [true; false]. Proof. reflexivity. Qed.
+  Goal testAccess (size := 3) (ARRAY {R; R}) (Const type (2'b"00")) [true; true]. Proof. reflexivity. Qed.
+  Goal testAccess (size := 3) (ARRAY {R; R}) (Const type (2'b"10")) [false; true]. Proof. reflexivity. Qed.
+  Goal testAccess (size := 3) (ARRAY {R; R}) (Const type (2'b"11")) [true; true]. Proof. reflexivity. Qed.
 
   Close Scope kami_expr.
   Opaque wlt_dec.
