CompletionBuffer/Ifc.v
@@ -1,0 +1,49 @@
+Require Import Kami.AllNotations.
+
+Section Ifc.
+  Class Params :=
+    { name: string;
+      size: nat;
+      inReqK: Kind;
+      outReqK: Kind;
+      storeReqK: Kind;
+      immResK: Kind;
+      resK: Kind;
+      inReqToOutReq: forall {ty}, inReqK @# ty -> outReqK @# ty;
+      inReqToStoreReq: forall {ty}, inReqK @# ty -> storeReqK @# ty;
+      isError: forall {ty}, immResK @# ty -> Bool @# ty;
+      isSend: forall {ty}, inReqK @# ty -> Bool @# ty;
+    }.
+  
+  Context {params: Params}.
+
+  Definition OutReq := STRUCT_TYPE {
+                           "tag"    :: Bit (Nat.log2_up size) ;
+                           "outReq" :: outReqK
+                         }.
+
+  Definition InRes := STRUCT_TYPE {
+                          "tag" :: Bit (Nat.log2_up size) ;
+                          "res" :: resK
+                        }.
+
+  Definition OutRes := STRUCT_TYPE {
+                           "storeReq" :: storeReqK ;
+                           "immRes"   :: immResK ;
+                           "res"      :: resK
+                         }.
+
+  Definition Store := STRUCT_TYPE {
+                          "storeReq" :: storeReqK ;
+                          "immRes"   :: immResK
+                        }.
+
+  Record Ifc: Type :=
+    {
+      regs: list RegInitT;
+      regFiles: list RegFileBase;
+      sendReq (memReq: forall ty, ty OutReq -> ActionT ty (Maybe immResK)) ty: ty inReqK -> ActionT ty Bool;
+      callback: forall {ty}, ty InRes -> ActionT ty Void;
+      callbackRule (callback: forall {ty}, ty OutRes -> ActionT ty Void): forall {ty}, ActionT ty Void;
+    }.
+End Ifc.
