Fetcher/Impl.v
@@ -1,0 +1,215 @@
+Require Import Kami.AllNotations.
+Require Import StdLibKami.Fifo.Ifc.
+Require Import StdLibKami.Fetcher.Ifc.
+
+Section Impl.
+  Context {ifcParams: Params}.
+      
+  Local Definition ShortVAddr := Bit (vAddrSz - 2).
+
+  Local Definition TopEntry: Kind
+    := STRUCT_TYPE {
+         "vaddr"  :: ShortVAddr;
+         "immRes" :: immResK;
+         "error"  :: finalErrK;
+         "upper"  :: Maybe CompInst;
+         "lower"  :: Maybe CompInst
+       }.
+
+  Local Instance fifoParams
+    :  Fifo.Ifc.Params
+    := {|
+         Fifo.Ifc.name := (name ++ ".fifo")%string;
+         Fifo.Ifc.k    := InRes;
+         Fifo.Ifc.size := size
+       |}.
+
+  Context (fifo: @Fifo.Ifc.Ifc fifoParams).
+
+  Local Definition topRegName := (Fetcher.Ifc.name ++ ".topReg")%string.
+  Local Definition outstandingName := (Fetcher.Ifc.name ++ ".outstanding")%string.
+  Local Definition clearOutstandingName := (Fetcher.Ifc.name ++ ".clearOutstanding")%string.
+
+  Local Open Scope kami_expr.
+  Local Open Scope kami_action.
+
+  Local Definition toVAddr ty (a: ShortVAddr @# ty) := ZeroExtendTruncMsb vAddrSz ({< a, $$(natToWord 2 0) >}).
+  
+  Local Definition isFull ty: ActionT ty Bool :=
+    Read outstanding: Bit lgSize <- outstandingName;
+    LETA numFree <- Fifo.Ifc.numFree fifo;
+    Ret (#outstanding < #numFree).
+
+  Local Definition canClear ty: ActionT ty Bool :=
+    Read clearOutstanding: Bit lgSize <- clearOutstandingName;
+    Ret (#clearOutstanding == $0).
+
+  Local Definition clear ty: ActionT ty Void :=
+    LETA _ <- Fifo.Ifc.flush fifo;
+    Read outstanding: Bit lgSize <- outstandingName;
+    Write clearOutstandingName: Bit lgSize <- #outstanding;
+    Write topRegName: TopEntry <- $$(getDefaultConst TopEntry);
+    Retv.
+
+  Local Definition isNextAddr ty (topAddr: ShortVAddr @# ty) (ftopAddr: VAddr @# ty) :=
+    (topAddr + $1) == (ZeroExtendTruncMsb (vAddrSz - 2) ftopAddr).
+  
+  Local Definition isNotComplete
+    ty
+    (top : TopEntry @# ty)
+    (ftop : Maybe InRes @# ty)
+    : ActionT ty Bool :=
+    Ret (! (isImmErr (top @% "immRes") || isFinalErr (top @% "error"))
+         && (top @% "upper" @% "valid")
+         && !(top @% "lower" @% "valid")
+         && !(isCompressed (top @% "upper" @% "data"))
+         && !((ftop @%"valid") && isNextAddr (top @% "vaddr") (ftop @% "data" @% "vaddr"))).
+
+  Local Definition notCompleteDeqRule ty: ActionT ty Void :=
+    Read top: TopEntry <- topRegName;
+    LETA ftop: Maybe InRes <- @Fifo.Ifc.first _ fifo _;
+    LETA notComplete <- isNotComplete #top #ftop;
+    If #notComplete && #ftop @% "valid" && !(isNextAddr (#top @% "vaddr" + $1) (#ftop @% "data" @% "vaddr"))
+    then @Fifo.Ifc.deq _ fifo _;
+    Retv.
+
+  Local Definition isAligned ty (vaddr: VAddr @# ty) := ZeroExtendTruncLsb 2 vaddr == $0.
+
+  Local Definition transferRule ty: ActionT ty Void :=
+    LETA isEmp: Bool <- @Fifo.Ifc.isEmpty _ fifo _;
+    Read top: TopEntry <- topRegName;
+    If !(#top @% "upper" @% "valid") && !#isEmp
+    then (
+      LETA deqValM: Maybe InRes <- @Fifo.Ifc.deq _ fifo _;
+      LET deqVal: InRes <- #deqValM @% "data";    
+      LET lower <- STRUCT { "valid" ::= isAligned (#deqVal @% "vaddr") ;
+                            "data"  ::= UniBit (TruncLsb _ _) (#deqVal @% "inst") };
+      LET topEntry
+        :  TopEntry
+        <- STRUCT {
+             "vaddr"  ::= ZeroExtendTruncMsb (vAddrSz - 2) (#deqVal @% "vaddr");
+             "immRes" ::= #deqVal @% "immRes";
+             "error"  ::= #deqVal @% "error";
+             "upper"  ::= Valid (UniBit (TruncMsb _ _) (#deqVal @% "inst"));
+             "lower"  ::= #lower};
+      Write topRegName: TopEntry <- #topEntry;
+      Retv );
+    Retv.
+
+  Local Definition callback ty (res: ty InRes): ActionT ty Void :=
+    Read clearOutstanding: Bit lgSize <- clearOutstandingName;
+    If #clearOutstanding == $0
+    then (LETA _ <- @Fifo.Ifc.enq _ fifo _ res; Retv)
+    else (Write clearOutstandingName : Bit lgSize <- #clearOutstanding - $1; Retv);
+    Read outstanding: Bit (Nat.log2_up size) <- outstandingName;
+    Write outstandingName <- #outstanding - $1;
+    Retv.
+
+  Local Definition sendAddr (sendReq : forall ty, ty OutReq -> ActionT ty Bool) ty (req: ty OutReq) :=
+    LETA retval <- sendReq _ req;
+    Read outstanding: Bit (Nat.log2_up size) <- outstandingName;
+    Write outstandingName <- #outstanding + IF #retval then $1 else $0;
+    Ret #retval.
+
+  Local Definition isStraddle ty (top: TopEntry @# ty) :=
+    !(top @% "lower" @% "valid") && !isCompressed (top @% "upper" @% "data").
+
+  Local Definition first ty: ActionT ty (Maybe OutRes) :=
+    Read top: TopEntry <- topRegName;
+    LETA ftopM: Maybe InRes <- (@Fifo.Ifc.first _ fifo _);
+    LETA notComplete : Bool <- isNotComplete #top #ftopM;
+    LET ftop <- #ftopM @% "data";
+
+    LET upperTopCompressed <- isCompressed (#top @% "upper" @% "data");
+           
+    LET retAddr: VAddr <-
+      (IF isImmErr (#top @% "immRes") || isFinalErr (#top @% "error")
+       then (IF #top @% "lower" @% "valid"
+             then toVAddr (#top @% "vaddr")
+             else (toVAddr (#top @% "vaddr")) + $2)
+       else (IF #top @% "lower" @% "valid"
+             then toVAddr (#top @% "vaddr")
+             else (IF #upperTopCompressed
+                   then (toVAddr (#top @% "vaddr")) + $2
+                   else (IF #notComplete
+                         then toVAddr (#top @% "vaddr" + $1)
+                         else (toVAddr (#top @% "vaddr")) + $2))));
+
+    LET retInst: Inst <-
+      (IF #top @% "lower" @% "valid"
+       then {< #top @% "upper" @% "data", #top @% "lower" @% "data" >}
+       else (IF #upperTopCompressed
+             then {< $0, #top @% "upper" @% "data" >}
+             else {< UniBit (TruncLsb compInstSz compInstSz) (#ftop @% "inst"), #top @% "upper" @% "data" >}));
+
+    LET straddle: Bool <- isStraddle #top;
+    
+    LET upperOnly: Bool <- (IF #top @% "lower" @% "valid"
+                            then $$ false
+                            else (IF #upperTopCompressed
+                                  then $$ true
+                                  else $$ false));
+    
+    LET pickFifo: Bool <- (IF #straddle
+                           then !(isImmErr (#top @% "immRes") || (isFinalErr (#top @% "error")))
+                           else $$false);
+
+    LET ret: OutRes <- STRUCT { "notComplete?" ::= #notComplete;
+                                "vaddr" ::= #retAddr;
+                                "immRes" ::= (IF #pickFifo then #ftop @% "immRes" else #top @% "immRes");
+                                "error" ::= (IF #pickFifo then #ftop @% "error" else #top @% "error");
+                                "compressed?" ::= isCompressed (UniBit (TruncLsb compInstSz compInstSz) #retInst);
+                                "errUpper?" ::= #pickFifo;
+                                "inst"  ::= #retInst};
+    Ret (STRUCT { "valid" ::= #top @% "upper" @% "valid";
+                  "data" ::= #ret}: Maybe OutRes @# ty).
+
+  Local Definition deq ty: ActionT ty Bool :=
+    Read top: TopEntry <- topRegName;
+    LETA ftopM: Maybe InRes <- (@Fifo.Ifc.first _ fifo _);
+    LETA notComplete : Bool <- isNotComplete #top #ftopM;
+    LET ftop <- #ftopM @% "data";
+
+    LET allowDeq <-
+      #top @% "upper" @% "valid" &&
+      ((isImmErr (#top @% "immRes") || isFinalErr (#top @% "error")) ||
+       (#top @% "lower" @% "valid" && !isCompressed (#top @% "lower" @% "data")) ||
+       (!(#top @% "lower" @% "valid") && !#notComplete));
+
+    LET newLowerValid <- #ftopM @% "valid" && (isAligned (#ftop @% "vaddr")) && !(isStraddle #top);
+
+    LET newTopRegDeq: TopEntry <- STRUCT { "vaddr"  ::= ZeroExtendTruncMsb (vAddrSz - 2) (#ftop @% "vaddr");
+                                           "immRes" ::= #ftop @% "immRes";
+                                           "error"  ::= #ftop @% "error";
+                                           "upper"  ::= STRUCT { "valid" ::= #ftopM @% "valid";
+                                                                 "data" ::= UniBit (TruncMsb compInstSz _)
+                                                                                   (#ftop @% "inst")};
+                                           "lower"  ::= STRUCT { "valid" ::= #newLowerValid;
+                                                                 "data" ::= UniBit (TruncLsb compInstSz _)
+                                                                                   (#ftop @% "inst")}
+                                         };
+
+    LET newTopRegLower: TopEntry <- #top @%[ "lower" <- STRUCT { "valid" ::= $$false;
+                                                                 "data" ::= $$(getDefaultConst (Bit compInstSz)) }];
+    Write topRegName <- IF #allowDeq then #newTopRegDeq else IF isCompressed (#top @% "lower" @% "data") then #newTopRegLower else #top;
+    Ret #allowDeq.
+
+  Local Definition regs
+    := (makeModule_regs
+          ((Register topRegName : TopEntry <- Default)
+             ++ (Register outstandingName : Bit lgSize <- Default)
+             ++ (Register clearOutstandingName : Bit lgSize <- Default))%kami ++
+       (@Fifo.Ifc.regs _ fifo)).
+
+  Definition impl: Ifc := {| Fetcher.Ifc.regs := regs;
+                             Fetcher.Ifc.regFiles := Fifo.Ifc.regFiles fifo;
+                             Fetcher.Ifc.isFull := isFull;
+                             Fetcher.Ifc.sendAddr := sendAddr;
+                             Fetcher.Ifc.callback := callback;
+                             Fetcher.Ifc.deq := deq;
+                             Fetcher.Ifc.first := first;
+                             Fetcher.Ifc.canClear := canClear;
+                             Fetcher.Ifc.clear := clear;
+                             Fetcher.Ifc.notCompleteDeqRule := notCompleteDeqRule;
+                             Fetcher.Ifc.transferRule := transferRule; |}.
+End Impl.
