RegArray/Ifc.v
@@ -1,0 +1,18 @@
+Require Import Kami.AllNotations.
+Require Import String.
+
+Section Ifc.
+  Class Params := { name : string ;
+                    k    : Kind ;
+                    size : nat ;
+                    init : option (ConstT k)
+                  }.
+
+  Context {params: Params}.
+
+  Record Ifc := { regs: list RegInitT;
+                  regFiles: list RegFileBase;
+                  read ty (idx: ty (Bit (Nat.log2_up size))): ActionT ty k;
+                  write ty (writeRq: ty (WriteRq (Nat.log2_up size) k)): ActionT ty Void;
+                }.
+End Ifc.
