RegArray/Impl.v
@@ -1,0 +1,34 @@
+Require Import Kami.AllNotations.
+Require Import StdLibKami.RegArray.Ifc.
+
+
+Section Impl.
+  Context {ifcParams: Ifc.Params}.
+
+  Local Notation Idx := (Bit (Nat.log2_up size)).
+
+  Local Open Scope kami_expr.
+  Local Open Scope kami_action.
+
+  Local Definition names := map (fun i => name ++ "_" ++ natToHexStr i)%string (seq 0 size).
+
+  Local Definition read ty (idx: ty Idx) : ActionT ty k :=
+   GatherActions (map (fun '(i, reg) => Read val: k <- reg;
+                      Ret (IF ($i == #idx)
+                           then #val else $$(getDefaultConst k))) (tag names)) as vals;
+   Ret (Kor vals).
+
+  Local Definition write ty (writeRq: ty (WriteRq (Nat.log2_up size) k)): ActionT ty Void :=
+    GatherActions (map (fun '(i, reg) => Read val: k <- reg;
+                                         Write reg: k <- (IF $i == #writeRq @% "addr" then #writeRq @% "data" else #val);
+                                         Retv) (tag names)) as _;
+    Retv.
+
+  Definition impl := {| regs := map (fun i => (i, existT RegInitValT (SyntaxKind k) match init with
+                                                                                    | None => None
+                                                                                    | Some x => Some (SyntaxConst x)
+                                                                                    end)) names;
+                        regFiles := nil;
+                        Ifc.read := read;
+                        Ifc.write := write |}.
+End Impl.
