Router/Ifc.v
@@ -1,0 +1,31 @@
+Require Import Kami.AllNotations.
+
+Section Ifc.
+  Record DeviceIfc (reqK respK: Kind): Type :=
+    {
+      deviceReq: forall {ty}, ty reqK -> ActionT ty Bool;
+      devicePoll: forall {ty}, ActionT ty (Maybe respK)
+    }.
+
+  Class Params :=
+    {
+      name: string;
+      reqK: Kind;
+      respK: Kind;
+      devices: list (DeviceIfc reqK respK);
+      numDevices := length devices;
+    }.
+
+  Context {params: Params}.
+
+  Definition OutReq := STRUCT_TYPE { "dtag" :: Bit (Nat.log2_up numDevices) ;
+                                     "req" :: reqK }.
+
+  Record Ifc :=
+    {
+      regs: list RegInitT;
+      regFiles: list RegFileBase;
+      sendReq: forall ty, ty OutReq -> ActionT ty Bool;
+      pollRules (callback: forall {ty}, ty respK -> ActionT ty Void): list (forall {ty}, ActionT ty Void);
+    }.
+End Ifc.
